Ughhhh well-founded recursion not working

theories/system_f.v
@@ -60,7 +60,7 @@ Module System_F.
   Inductive step : expr -> expr -> Prop :=
   | cbv_efun e1 e2 e1' : e1 ⇒ e1' -> (EApp e1 e2) ⇒ (EApp e1' e2)
   | cbv_earg t e e2 e2' : e2 ⇒ e2' -> (EApp (EAbs t e) e2) ⇒ (EApp (EAbs t e) e2')
-  | cbv_esub t e v : EApp (EAbs t e) v ⇒ (e.[v/])
+  | cbv_esub t e v : value v -> EApp (EAbs t e) v ⇒ (e.[v/])
   | cbv_tfun e e' t : e ⇒ e' -> (TApp e t) ⇒ (TApp e' t)
   | cbv_tsub e t : TApp (TAbs e) t ⇒ e.|[t/]
   where " e '⇒' f " := (step e f).
@@ -98,14 +98,10 @@ Module System_F.
   Definition rel : Type := Relation_Definitions.relation expr.
 
   (* A compatible relation is a binary relation that respects beta equivalence *)
-  Definition compatible (R : rel) : Prop :=
-    forall e1 e2 e1' e2', e1 ≡ e1' -> e2 ≡ e2' -> R e1 e2 -> R e1' e2'.
+  Definition compatible (R : rel) : Prop := forall v1 v2, R v1 v2 -> (value v1 /\ value v2).
 
   (* A dependent sum of relation with a proof of compatibility *)
   Definition compat_rel : Type := sig compatible.
-
-  Lemma beta_equiv_compatible : compat_rel.
-  Proof. exists beta_equiv. unfold compatible. intros. apply rst_trans with (y := e1); eauto. Qed.
 
   Fixpoint V (ρ : var -> compat_rel) t v1 v2 {struct t} : Prop :=
     let E ρ t e1 e2 : Prop := exists v1 v2, e1 ⇒* v1 /\ e2 ⇒* v2 /\ V ρ t v1 v2 in
@@ -113,7 +109,7 @@ Module System_F.
     | TVar n => proj1_sig (ρ n) v1 v2
     | Unit => v1 = Null /\ v2 = Null
     | Arrow t1 t2 => exists (e1 e2 : {bind expr}), v1 = EAbs t1 e1 /\ v2 = EAbs t1 e2 /\ (forall v1' v2', V ρ t1 v1' v2' -> E ρ t2 (e1.[v1'/]) (e2.[v2'/]))
-    | All t => exists e1 e2 : expr, v1 = TAbs e1 /\ v2 = TAbs e2 /\ (forall R, E (R .: ρ) t e1 e2)
+    | All t => exists e1 e2 : {bind tipe in expr}, v1 = TAbs e1 /\ v2 = TAbs e2 /\ (forall R, E (R .: ρ) t e1 e2)
     end.
 
   Definition E ρ t e1 e2 : Prop := exists v1 v2, e1 ⇒* v1 /\ e2 ⇒* v2 /\ V ρ t v1 v2.
@@ -122,18 +118,22 @@ Module System_F.
   Proof. intros. unfold E. eauto. Qed.
   #[export] Hint Resolve V_implies_E : core.
 
-  (* Lemma V_implies_value : forall ρ t v1 v2, (forall n, t <> TVar n) -> V ρ t v1 v2 -> value v1 /\ value v2. *)
-  (* Proof. *)
-  (*   intros ρ t v1 v2 H0 H. induction t. *)
-  (*   - destruct H. subst. smash. *)
-  (*   - destruct H as [e1 [e2 [a1 [a2 _]]]]. subst. smash. *)
-  (*   - specialize (H0 v). contradiction. *)
-  (*   - assert (forall n, t <> TVar n) as A. { intros. unfold not. intros. subst. } *)
+  Lemma V_implies_value : forall ρ t v1 v2, V ρ t v1 v2 -> value v1 /\ value v2.
+  Proof.
+    intros ρ t v1 v2 H. generalize dependent ρ. induction t; intros.
+    - destruct H. subst. smash.
+    - destruct H as [e1 [e2 [a1 [a2 _]]]]. subst. smash.
+    - unfold V in H. remember (ρ v) as R. destruct R. simpl in H. unfold compatible in c. apply c in H. assumption.
+    - simpl in H. destruct H as [e1 [e2 [Eq1 [Eq2 Hyp]]]]. subst. smash.
+  Qed.
+
+  Corollary V_is_compatible : forall ρ t, compatible (V ρ t).
+  Proof. unfold compatible. intros. eapply V_implies_value. eauto. Qed.
 
   (* The free expression variable context is a stack, with the head being the most recently bound variable *)
   Definition ev_context : Type := List.list tipe.
 
-  (** Since we're using de Bruijn indices, the type context just limits how many type variables you can have *)
+  (* Since we're using de Bruijn indices, the type context just limits how many type variables you can have *)
   Definition tv_context : Type := nat.
 
   Definition lookup : ev_context -> nat -> option tipe := @nth_error tipe.
@@ -152,7 +152,7 @@ Module System_F.
 
   Reserved Notation " Δ ';' Γ '⊢' e ':::' t " (at level 96).
   Inductive typing : tv_context -> ev_context -> expr -> tipe -> Prop :=
-  | arrow_intro Δ Γ e t1 t2 : well_formed_tipe Δ t1 -> Δ;(t1 :: Γ) ⊢ e ::: t2 -> Δ;Γ ⊢ (EAbs t1 e) ::: (t1 → t2)
+  | arrow_intro Δ Γ e t1 t2 : Δ;(t1 :: Γ) ⊢ e ::: t2 -> Δ;Γ ⊢ (EAbs t1 e) ::: (t1 → t2)
   | arrow_elim Δ Γ e1 e2 t1 t2 : Δ;Γ ⊢ e1 ::: (t1 → t2) -> Δ;Γ ⊢ e2 ::: t1 -> Δ;Γ ⊢ (EApp e1 e2) ::: t2
   | all_intro Δ Γ e t : (S Δ);Γ ⊢ e ::: t -> Δ;Γ ⊢ (TAbs e) ::: (All t)
   | all_elim Δ Γ e t1 t2 : Δ;Γ ⊢ e ::: (All t1) -> Δ;Γ ⊢ (TApp e t2) ::: t1.[t2/]
@@ -169,9 +169,25 @@ Module System_F.
   Proof. intros. induction H; eauto. Qed.
   #[export] Hint Resolve app_arg_steps_steps : core.
 
-  Lemma tapp_fun_steps_steps :  forall e e' t, e ⇒* e' -> (TApp e t) ⇒* (TApp e' t).
+  Lemma tapp_fun_steps_steps : forall e e' t, e ⇒* e' -> (TApp e t) ⇒* (TApp e' t).
   Proof. intros. induction H; eauto. Qed.
   #[export] Hint Resolve tapp_fun_steps_steps : core.
+
+  Lemma tipe_subst_value_value : forall v t, value v -> value v.|[t/].
+  Proof. intros. induction H; simpl; eauto. Qed.
+  #[export] Hint Resolve tipe_subst_value_value : core.
+
+  Lemma tipe_subst_commutes_with_step : forall e e' t, e ⇒ e' -> e.|[t/] ⇒ e'.|[t/].
+  Proof.
+    intros. induction H; simpl; eauto.
+    - apply (tipe_subst_value_value v t) in H. assert ((e.|[t/]).[(v.|[t/])/] = e.[v/].|[t/]). { autosubst. } rewrite <- H0. eauto.
+    - assert (e.|[t0/].|[t/] = e.|[up (t .: ids)].|[t0.[t/]/]). { autosubst. } simpl. simpl in H. rewrite H. eauto.
+  Qed.
+  #[export] Hint Resolve tipe_subst_commutes_with_step : core.
+
+  Lemma tipe_subst_commutes_with_steps : forall e e' t, e ⇒* e' -> e.|[t/] ⇒* e'.|[t/].
+  Proof. intros. induction H; eauto. Qed.
+  #[export] Hint Resolve tipe_subst_commutes_with_steps : core.
 
   (* This is the expression Λ X. λ x:X. x *)
   Example polymorphic_identity : expr :=
@@ -185,25 +201,56 @@ Module System_F.
 
   Definition parallel_subst : Type := var -> expr.
 
+  Inductive good_rel_substs : tv_context -> (var -> compat_rel) -> Prop :=
+  | nil_good_rel_substs ρ : good_rel_substs 0 ρ
+  | cons_good_re_substs Δ ρ R : good_rel_substs Δ ρ -> good_rel_substs (S Δ) (R .: ρ).
+
   Inductive sem_rel_expr_substs : ev_context -> (var -> compat_rel) -> parallel_subst -> parallel_subst -> Prop :=
   | nil_sem_rel_expr_substs ρ : sem_rel_expr_substs nil ρ ids ids
   | cons_sem_rel_expr_substs ρ t Γ γ1 γ2 v1 v2 : sem_rel_expr_substs Γ ρ γ1 γ2 -> V ρ t v1 v2 -> sem_rel_expr_substs (t :: Γ) ρ (v1 .: γ1) (v2 .: γ2).
   #[export] Hint Constructors sem_rel_expr_substs : core.
 
-  Definition semantically_related (Δ : tv_context) Γ e1 e2 t :=
-    forall ρ γ1 γ2, sem_rel_expr_substs Γ ρ γ1 γ2 -> E ρ t e1 .[γ1] e2.[γ2].
+  Definition semantically_related (Δ : tv_context) Γ e1 e2 t := forall ρ γ1 γ2,
+      good_rel_substs Δ ρ -> sem_rel_expr_substs Γ ρ γ1 γ2 -> E ρ t e1.[γ1] e2.[γ2].
   Notation "Δ ';' Γ ⊨ e '~' f ':::' t" := (semantically_related Δ Γ e f t) (at level 96).
 
   Lemma autosubst_help : forall e γ v, e.[up γ].[v/] = e.[v .: γ].
   Proof. intros. autosubst. Qed.
 
-  Lemma sem_rel_expr_substs_prepend : forall Γ ρ γ1 γ2 (R : compat_rel),
-      sem_rel_expr_substs Γ ρ γ1 γ2 ->
-      sem_rel_expr_substs Γ (R .: ρ) (γ1 >>| ren(+1)) (γ2 >>| ren(+1)).
+  (* Lemma V_prepend : forall ρ R t v1 v2, V ρ t v1 v2 -> V (R .: ρ) t v1.|[ren (+1)] v2.|[ren (+1)]. *)
+  (* Proof. *)
+  (*   intros. generalize dependent ρ. intros.  *)
+
+  (* Lemma sem_rel_expr_substs_prepend : forall Γ ρ γ1 γ2 (R : compat_rel), *)
+  (*     sem_rel_expr_substs Γ ρ γ1 γ2 -> *)
+  (*     sem_rel_expr_substs Γ (R .: ρ) (γ1 >>| ren(+1)) (γ2 >>| ren(+1)). *)
+  (* Proof. *)
+  (*   intros. induction H. *)
+  (*   - eauto. *)
+  (*   - simpl. *)
+  (*     assert (scons (v1.|[ren (lift 1)]) (hcomp γ1 (ren (lift 1))) = (hcomp (scons v1 γ1) (ren (lift 1)))). { autosubst. } *)
+  (*     assert (scons (v2.|[ren (lift 1)]) (hcomp γ2 (ren (lift 1))) = (hcomp (scons v2 γ2) (ren (lift 1)))). { autosubst. } *)
+  (*     rewrite <- H1. rewrite <- H2. *)
+  (*     apply cons_sem_rel_expr_substs; eauto. *)
+  (* Admitted. *)
+
+(*   The lemma says syntactically substituting some type for α in τ and then in- *)
+(* terpreting it is the same as semantically substituting the type for α. *)
+  Lemma compositionality : forall Δ t t' ρ v1 v2,
+      well_formed_tipe (S Δ) t ->
+      V ((exist compatible (V ρ t') (V_is_compatible ρ t')) .: ρ) t v1 v2 ->
+      V ρ t.[t'/] v1.|[t'/] v2.|[t'/].
+  Admitted.
+  (* Proof. *)
+  (*   intros. induction t. *)
+  (*   - split; simpl in H1; destruct H1; subst; smash. *)
+  (*   - simpl. simpl in H1. inversion H0. specialize (IHt1 H5). specialize (IHt2 H6). destruct H1 as [e1 [e2 [Eq1 [Eq2 Hmm]]]]. subst. simpl. exists e1.|[t'/], e2.|[t'/]; smash. intros. simpl in IHt1. simpl in IHt1. assert (V (exist compatible (V ρ t') (V_is_compatible ρ t') .: ρ) t1 v1' v2'). *)
+
+  Lemma well_formed_vars_values : forall Γ ρ n γ1 γ2 t, lookup Γ n = Some t -> sem_rel_expr_substs Γ ρ γ1 γ2 -> V ρ t (γ1 n) (γ2 n).
   Proof.
-    intros. induction H.
-    - eauto.
-    - Unset Printing Notations. Print hcomp. assert ((scons v1 (hcomp γ1 (ren (lift 1)))) = (hcomp (scons v1 γ1) (ren (lift 1)))).
+    intros. unfold lookup in H. induction H0.
+    - destruct n; intros; inversion H.
+    - induction n. admit.
   Admitted.
 
   (** Fundamental theorem of logical relations for System F : Parametricity *)
@@ -211,20 +258,19 @@ Module System_F.
   Proof.
     intros. unfold semantically_related. unfold E. induction H; intros.
     (* EAbs *)
-    - exists (EAbs t1 e.[up γ1]), (EAbs t1 e.[up γ2]). smash. exists e.[up γ1], e.[up γ2]. smash. intros. specialize (IHtyping ρ (v1' .: γ1) (v2' .: γ2)). repeat rewrite autosubst_help. auto.
+    - simpl. exists (EAbs t1 e.[up γ1]), (EAbs t1 e.[up γ2]). smash. exists e.[up γ1], e.[up γ2]. smash. intros. specialize (IHtyping ρ (v1' .: γ1) (v2' .: γ2)). repeat rewrite autosubst_help. auto.
     (* EApp *)
-    - simpl. destruct (IHtyping1 ρ γ1 γ2 H1) as [f1 [f2 [Sfun1 [Sfun2 Vfun]]]]. destruct (IHtyping2 ρ γ1 γ2 H1) as [arg1 [arg2 [Sarg1 [Sarg2 Varg]]]]. clear IHtyping1. clear IHtyping2. inversion Vfun. rename x into e3. destruct H2 as [e4 [Eq1 [Eq2]]]. subst. specialize (H2 arg1 arg2 Varg). destruct H2 as [v1 [v2 [Sapp1 [Sapp2 Vapp]]]]. exists v1, v2. smash.
-      + apply multistep_trans with (e' := e3.[arg1/]); eauto. apply multistep_trans with (e' := EApp (EAbs t1 e3) e2.[γ1]); eauto.
-      + apply multistep_trans with (e' := e4.[arg2/]); eauto. apply multistep_trans with (e' := EApp (EAbs t1 e4) e2.[γ2]); eauto.
+    - simpl. destruct (IHtyping1 ρ γ1 γ2 H1 H2) as [f1 [f2 [Sfun1 [Sfun2 Vfun]]]]. destruct (IHtyping2 ρ γ1 γ2 H1 H2) as [arg1 [arg2 [Sarg1 [Sarg2 Varg]]]]. clear IHtyping1. clear IHtyping2. inversion Vfun. rename x into e3. destruct H3 as [e4 [Eq1 [Eq2]]]. subst. specialize (H3 arg1 arg2 Varg). destruct H3 as [v1 [v2 [Sapp1 [Sapp2 Vapp]]]]. exists v1, v2. smash.
+      + apply multistep_trans with (e' := e3.[arg1/]); eauto. apply multistep_trans with (e' := EApp (EAbs t1 e3) e2.[γ1]); eauto. apply V_implies_value in Varg. destruct Varg. apply multistep_trans with (e' := EApp (EAbs t1 e3) arg1); eauto.
+      + apply multistep_trans with (e' := e4.[arg2/]); eauto. apply multistep_trans with (e' := EApp (EAbs t1 e4) e2.[γ2]); eauto. apply V_implies_value in Varg. destruct Varg. apply multistep_trans with (e' := EApp (EAbs t1 e4) arg2); eauto.
     (* TAbs *)
-    - exists (TAbs e).[γ1], (TAbs e).[γ2]. smash. simpl. exists (e.[γ1 >>| ren (+1)]), (e.[γ2 >>| ren (+1)]). smash. intros. specialize (IHtyping (R .: ρ) (γ1 >>| ren (+1)) (γ2 >>| ren (+1))). Unset Printing Notations. admit.
+    - exists (TAbs e).[γ1], (TAbs e).[γ2]. smash. simpl. exists (e.[γ1 >>| ren (+1)]), (e.[γ2 >>| ren (+1)]). smash. intros. specialize (IHtyping (R .: ρ) (γ1 >>| ren (+1)) (γ2 >>| ren (+1))). admit.
     (* TApp *)
-    - destruct (IHtyping ρ γ1 γ2 H0) as [v1 [v2 [S1 [S2 Vall]]]]. inversion Vall as [e1 [e2 [Eq1 [Eq2]]]]. subst.
-
-  (** Strong normalization of CBV STLC *)
-  Theorem strong_normalization : forall e t, ∅ ⊢ e ::: t -> exists v, value v /\ e ⇒* v.
-  Proof.
-    intros. apply (fundamental_theorem nil e t) in H. unfold semant_typing in H. specialize H with (@ids expr Ids_expr). rewrite subst_id in H. destruct H. apply subst_empty. exists x. split; destruct H; (try apply (V_implies_value t); auto).
-  Qed.
+    - destruct (IHtyping ρ γ1 γ2 H0 H1) as [v1 [v2 [S1 [S2 Vall]]]]. simpl. inversion Vall as [e1 [e2 [Eq1 [Eq2]]]]. subst. destruct (H2 (exist compatible (V ρ t2) (V_is_compatible ρ t2))) as [v1 [v2 [SS1 [SS2 Vsub]]]]. exists v1.|[t2/], v2.|[t2/]. repeat split.
+      + apply multistep_trans with (e' := TApp (TAbs e1) t2); eauto.
+      + apply multistep_trans with (e' := TApp (TAbs e2) t2); eauto.
+      + subst. apply (compositionality Δ); eauto. admit.
+    - exists Null, Null; smash.
+    - exists (γ1 n), (γ2 n). simpl. smash. apply (well_formed_vars_values Γ); eauto.
 
 End System_F.
